$$
\begin{cases}
	\vec l_1 = c_{11}\vec e_1 + ... + c_{n1}\vec e_n \\
	\vdots \\
	\vec l_n = c_{1m}\vec e_1 + ... + c_{nm}\vec e_n \\
\end{cases}
\begin{cases}
	\vec l^\prime_1 = c^\prime_{11}\vec {e^\prime}_1 + ... + c^\prime_{n1}\vec {e_n^\prime} \\
	\vdots \\
	\vec l^\prime_n = c^\prime_{1m}\vec {e_1^\prime} + ... + c^\prime_{nm}\vec {e_n^\prime} \\
\end{cases}
$$
$$\vec x = \alpha_1^\prime(e_{11}\vec e_1 + ... + c_{n1}\vec e_n) + ... + \alpha_n^\prime (c_{1n}\vec e_1 + ... + c_{nn}\vec e_n) = $$
$$
\vec e_1(\alpha_1^\prime c_{11} + ... + \alpha_n^\prime) + ... + \vec e_n(\alpha_1^\prime c_{n1} + ... + \alpha_n^\prime c_{nn})
$$

