#### $y = x^\mu, \mu \in \mathbb{R}$ 

##### вычисление [[производная|производной]] 
- $$\frac{\Delta y}{\Delta x} = \frac{(x + \Delta x)^\mu - x^\mu}{\Delta x} = x^{\mu - 1}\frac{(1 + \frac{\Delta x}{x})^\mu - 1}{\frac{\Delta x}{x}}$$
- $$\underset{\alpha \to 0}{\lim} = \frac{(1 + \frac{\Delta \alpha}{\alpha})^\mu - 1}{\frac{\Delta \alpha}{\alpha}} = \mu \Rightarrow$$
- $$x^{\mu - 1}\frac{(1 + \frac{\Delta x}{x})^\mu - 1}{\frac{\Delta x}{x}} = \mu x^{\mu - 1}$$
***
#формула #матанализ #производная 