#### $$f(x) = f(x_0) + f^\prime(x_0)(x - x_0) + \frac{f^{\prime\prime}(x_0)}{2!} + ... + \frac{f^{(n)}(x_0)}{n!}(x - x_0) + \frac{f^{(n+1)}(c)}{(n + 1)!}$$ где $c$ - точка между $x$ и $x_0$ 

##### вывод
$r_n(x) = f(x) - p_n(x)$ - остаток 
$f^{(n + 1)}(x_0)$ 
$z \in [x_0, x]$ функция непрерывна на $[x_0, x]$ 
$\varphi(z) = f(x) - f(z) - \frac{f^\prime(z)}{1!}(x - z) - ... -\frac{f^{(n)}(z)}{n!}(x - z)^n$ 
$\varphi(x_0) = r_0(x)$ - остаток, $\varphi(x) = 0$ 
$$\varphi^\prime(z) = -f^\prime(z) - [\frac{f^{\prime\prime}(z)}{1!} - f^\prime(z)] - [\frac{f^{\prime\prime\prime}(z)}{2!} - \frac{f^{\prime\prime}(z)}{1!}] - [\frac{f^{(n  + 1)}(z)}{n!} - \frac{f^{(n)}}{(n - 1)!}] = -\frac{f^{n + 1}(z)}{n!}(x - z)^n$$
- используем теорему коши 
$$\frac{\varphi(x) - \varphi(x_0)}{\psi(x) - \psi(x_0)} = \frac{\varphi^\prime(c)}{\psi^\prime(c)}$$
- $\psi(z) = (x - z)^{n + 1}$ 
	- $\psi^\prime (z) = -(n + 1)(x - z)^n$ 
	- $\psi(x_0) = (x-x_0)^{n + 1}$
	- $\psi(x) = 0$ 
- подставляем значения
- $$\frac{0 - r_n(x)}{0 - (x-x_0)} = \frac{\frac{-f^{n + 1}(c)(x-c)^n}{n!}}{-(n+1)(x-c)^n}$$
- $$\frac{r_n(x)}{(x-x_0)^{n + 1}} = \frac{f^{(n+1)}(c)}{(n + 1)!}$$
- $$r_n = \frac{f^{(n + 1)}(c)}{(n + 1)!}(x - x_0)^{n + 1}$$
***
#формула #матанализ #производная 